.

src/program_proof/session/session_definitions.v
@@ -2,45 +2,37 @@ From Perennial.program_proof.session Require Export session_prelude.
 From Goose.session Require server client.
 
 Module SessionServer := Goose.session.server.
+
 Module SessionClient := Goose.session.client.
 
-#[local] Tactic Notation "tac_val_t" :=
-  let val := lazymatch goal with [ |- val_ty (?val _) _ ] => val end in
-  lazymatch goal with [ v : tuple_of ?tv |- _ ] => unfold tuple_of in v; unfold tv in v; simpl in v; unfold val; simpl end;
-  repeat constructor; auto.
+Definition CONSTANT : Z :=
+  2 ^ 64 - 2.
 
-#[local] Tactic Notation "tac_IntoVal" integer( n ) :=
-  intros;
-  lazymatch goal with [ v : tuple_of ?tv |- _ ] => unfold tuple_of in v; unfold tv in v; simpl in v; simpl SessionPrelude.value_of; do n destruct v as [v ?]; simpl end;
-  repeat lazymatch goal with [ t : Slice.t |- _ ] => destruct t end; auto.
-
-#[universes(template)]
-Class has_value_boundary (t: Type) : Type :=
-  value_bound (a: Z) (object: t) : Prop.
-
-#[global] Hint Unfold value_bound : session_hints.
-
-#[global]
-Instance u64_has_value_boundary : has_value_boundary u64 :=
-  fun a: Z => fun u: u64 => a >= 1 /\ uint.Z u <= 2 ^ 64 - a.
-
-#[global]
-Instance nat_has_value_boundary : has_value_boundary nat :=
-  fun a: Z => fun n: nat => a >= 1 /\ uint.Z n <= 2 ^ 64 - a.
-
-Lemma u64_has_value_boundary_dec a n
-  : {u64_has_value_boundary a n} + {~ u64_has_value_boundary a n}.
+Lemma CONSTANT_unfold
+  : CONSTANT = 2 ^ 64 - 2.
 Proof.
-  unfold u64_has_value_boundary;
-  pose proof (Z.ge_dec a 1) as [YES_ge | NO_ge];
-  pose proof (Z.le_dec (uint.Z n) (2 ^ 64 - a)) as [YES_le | NO_le];
-  first [now left; split | right; word].
+  reflexivity.
 Qed.
 
-#[global]
-Instance list_has_value_boundary {t: Type} (t_has_value_boundary: has_value_boundary t) : has_value_boundary (list t) :=
-  let has_value_boundary : has_value_boundary t := t_has_value_boundary in
-  fun a: Z => Forall (has_value_boundary a).
+Lemma CONSTANT_minus_1
+  : CONSTANT - 1 = 18446744073709551613.
+Proof.
+  reflexivity.
+Qed.
+
+Definition nat_le_CONSTANT (n : nat) : Prop :=
+  Z.of_nat n <= CONSTANT.
+
+Definition u64_le_CONSTANT (u : u64) : Prop :=
+  uint.Z u <= CONSTANT.
+
+Lemma CONSTANT_ge_0
+  : u64_le_CONSTANT (W64 0).
+Proof.
+  red; unfold CONSTANT. word.
+Qed.
+
+#[global] Opaque CONSTANT.
 
 Module _Data.
 
@@ -67,7 +59,19 @@ Module _Data.
 
 End _Data.
 
-#[local] Opaque _Data.t.
+#[local] Tactic Notation "tac_val_t" :=
+  let val := lazymatch goal with [ |- val_ty (?val _) _ ] => val end in
+  lazymatch goal with [ v : tuple_of ?tv |- _ ] => unfold tuple_of in v; unfold tv in v; simpl in v; unfold val; simpl end;
+  repeat constructor; auto.
+
+#[local] Tactic Notation "tac_IntoVal" integer( n ) :=
+  intros;
+  lazymatch goal with [ v : tuple_of ?tv |- _ ] => unfold tuple_of in v; unfold tv in v; simpl in v; simpl SessionPrelude.value_of; do n destruct v as [v ?]; simpl end;
+  repeat lazymatch goal with [ t : Slice.t |- _ ] => destruct t end; auto.
+
+#[local] Tactic Notation "tac_IntoValForType" :=
+  let tv := lazymatch goal with [ |- IntoValForType (tuple_of ?tv) _ ] => tv end in
+  unfold tuple_of, tv, _Data.t; simpl; repeat split; auto.
 
 Module Operation.
 
@@ -87,22 +91,10 @@ Module Operation.
   Definition val (v: tuple_of tv) : val :=
     SessionPrelude.value_of v.
 
-  #[projections(primitive), universes(template)]
-  Record t {u64: Type} : Type := mk
+  Record t : Type := mk
     { VersionVector: list u64
     ; Data:          _Data.t
     }.
-
-  #[global] Arguments t : clear implicits. 
-
-  #[global]
-  Instance FMap
-    : FMap t.
-  Proof.
-    intros A B A_to_B F_A. econstructor.
-    - refine (fmap A_to_B _). refine (VersionVector _). exact F_A.
-    - refine (_). refine (Data _). exact F_A.
-  Defined.
 
   #[global, program]
   Instance IntoVal : IntoVal (tuple_of tv) :=
@@ -114,46 +106,58 @@ Module Operation.
     tac_IntoVal 1.
   Defined.
 
-  Section ADD_ON.
+  Theorem val_t v
+    : val_ty (Operation.val v) (struct.t SessionServer.Operation).
+  Proof.
+    tac_val_t.
+  Qed.
 
-  Context {u64: Type}.
+  #[global] Hint Resolve val_t : core.
+
+  #[global] Instance Session_IntoValForType
+    : IntoValForType (tuple_of tv) (struct.t SessionServer.Operation).
+  Proof.
+    tac_IntoValForType.
+  Qed.
+
+  #[global] Instance Client_IntoValForType
+    : IntoValForType (tuple_of tv) (struct.t SessionClient.Operation).
+  Proof.
+    tac_IntoValForType.
+  Qed.
+
+  Section ADD_ON.
 
   Section HASKELLISH_INSTANCES.
 
-  Definition getVersionVector (op: Operation.t u64) : list u64 :=
+  Definition getVersionVector (op: Operation.t) : list u64 :=
     op.(VersionVector).
 
-  Context {u64_well_formed: u64 -> Prop}.
-
-  Definition well_formed (n: nat) (op: Operation.t u64) : Prop :=
-    Forall u64_well_formed op.(VersionVector) /\ length op.(VersionVector) = n.
-
-  Context {u64_hsEq: SessionPrelude.hsEq u64 (well_formed := u64_well_formed)}.
+  Definition well_formed (n: nat) (op: Operation.t) : Prop :=
+    Forall (fun _ :  u64 => True) op.(VersionVector) /\ length op.(VersionVector) = n.
 
   #[global]
-  Instance hsEq (n: nat) : SessionPrelude.hsEq (Operation.t u64) (well_formed := well_formed n) :=
+  Instance hsEq (n: nat) : SessionPrelude.hsEq (Operation.t) (well_formed := well_formed n) :=
     SessionPrelude.hsEq_preimage getVersionVector.
 
-  Context {u64_hsOrd: SessionPrelude.hsOrd u64 (well_formed := u64_well_formed)}.
-
   #[global]
-  Instance hsOrd (n: nat) : SessionPrelude.hsOrd (Operation.t u64) (well_formed := well_formed n) :=
+  Instance hsOrd (n: nat) : SessionPrelude.hsOrd (Operation.t) (well_formed := well_formed n) :=
     SessionPrelude.hsOrd_preimage getVersionVector.
 
   End HASKELLISH_INSTANCES.
 
-  Definition size_of (object: t u64) : nat :=
-    length object.(VersionVector).
+  Definition size_of (op: Operation.t) : nat :=
+    length op.(VersionVector).
 
-  Context `(has_value_boundary u64).
-
-  #[global]
-  Instance value_bound : has_value_boundary (t u64) :=
-    fun a: Z => fun object: t u64 => value_bound a object.(VersionVector).
+  Definition value_bound (op: Operation.t) : Prop :=
+    Forall u64_le_CONSTANT op.(Operation.VersionVector).
 
   End ADD_ON.
 
 End Operation.
+
+#[global] Hint Unfold Operation.size_of : session_hints.
+#[global] Hint Unfold Operation.value_bound : session_hints.
 
 Module Message.
 
@@ -171,10 +175,9 @@ Module Message.
     end.
 
   Definition val (v: tuple_of tv) : val :=
-    SessionPrelude.value_of v.
+    tuple_of_has_value_of tv v.
 
-  #[projections(primitive), universes(template)]
-  Record t {u64: Type} : Type := mk
+  Record t : Type := mk
     { MessageType:  u64
 
     ; C2S_Client_Id:            u64
@@ -185,7 +188,7 @@ Module Message.
 
     ; S2S_Gossip_Sending_ServerId:   u64
     ; S2S_Gossip_Receiving_ServerId: u64
-    ; S2S_Gossip_Operations:         list (Operation.t u64)
+    ; S2S_Gossip_Operations:         list Operation.t
     ; S2S_Gossip_Index:              u64
 
     ; S2S_Acknowledge_Gossip_Sending_ServerId:   u64
@@ -199,33 +202,6 @@ Module Message.
     ; S2C_Client_Number:        u64
     }.
 
-  #[global] Arguments t : clear implicits.
-
-  #[global]
-  Instance FMap
-    : FMap t.
-  Proof.
-    intros A B A_to_B F_A. econstructor.
-    - refine (A_to_B _). refine (MessageType _). exact F_A.
-    - refine (A_to_B _). refine (C2S_Client_Id _). exact F_A.
-    - refine (A_to_B _). refine (C2S_Server_Id _). exact F_A.
-    - refine (A_to_B _). refine (C2S_Client_OperationType _). exact F_A.
-    - refine (_). refine (C2S_Client_Data _). exact F_A.
-    - refine (fmap A_to_B _). refine (C2S_Client_VersionVector _). exact F_A.
-    - refine (A_to_B _). refine (S2S_Gossip_Sending_ServerId _). exact F_A.
-    - refine (A_to_B _). refine (S2S_Gossip_Receiving_ServerId _). exact F_A.
-    - refine (fmap (Operation.FMap A B A_to_B) _). refine (S2S_Gossip_Operations _). exact F_A.
-    - refine (A_to_B _). refine (S2S_Gossip_Index _). exact F_A.
-    - refine (A_to_B _). refine (S2S_Acknowledge_Gossip_Sending_ServerId _). exact F_A.
-    - refine (A_to_B _). refine (S2S_Acknowledge_Gossip_Receiving_ServerId _). exact F_A.
-    - refine (A_to_B _). refine (S2S_Acknowledge_Gossip_Index _). exact F_A.
-    - refine (A_to_B _). refine (S2C_Client_OperationType _). exact F_A.
-    - refine (_). refine (S2C_Client_Data _). exact F_A.
-    - refine (fmap A_to_B _). refine (S2C_Client_VersionVector _). exact F_A.
-    - refine (A_to_B _). refine (S2C_Server_Id _). exact F_A.
-    - refine (A_to_B _). refine (S2C_Client_Number _). exact F_A.
-  Defined.
-
   #[global, program]
   Instance IntoVal : IntoVal (tuple_of tv) :=
     { to_val := val
@@ -236,42 +212,40 @@ Module Message.
     tac_IntoVal 17.
   Defined.
 
+  Theorem val_t v
+    : val_ty (Message.val v) (struct.t SessionServer.Message).
+  Proof.
+    tac_val_t.
+  Qed.
+
+  #[global] Hint Resolve val_t : core.
+
+  #[global] Instance Session_IntoValForType
+    : IntoValForType (tuple_of tv) (struct.t SessionServer.Message).
+  Proof.
+    tac_IntoValForType.
+  Qed.
+
+  #[global] Instance Client_IntoValForType
+    : IntoValForType (tuple_of tv) (struct.t SessionClient.Message).
+  Proof.
+    unfold tuple_of. unfold tv. unfold _Data.t. simpl. constructor; auto. simpl. repeat split; auto.
+  Qed.
+
   Section ADD_ON.
 
-  Context {u64: Type}.
+  Definition size_of (msg: Message.t) : nat * nat :=
+    (length msg.(C2S_Client_VersionVector), length msg.(S2C_Client_VersionVector)).
 
-  Definition size_of (object: t u64) : nat * nat :=
-    (length object.(C2S_Client_VersionVector), length object.(S2C_Client_VersionVector)).
-
-  Context `(has_value_boundary u64).
-
-  Variant _value_bound {a: Z} (object: t u64) : Prop :=
-    | _value_bound_intro
-      (MessageType_bound: value_bound 1 object.(MessageType))
-      (C2S_Client_Id_bound: value_bound a object.(C2S_Client_Id))
-      (C2S_Server_Id_bound: value_bound a object.(C2S_Server_Id))
-      (C2S_Client_OperationType_bound: value_bound 1 object.(C2S_Client_OperationType))
-      (C2S_Client_VersionVector: value_bound a object.(C2S_Client_VersionVector))
-      (S2S_Gossip_Sending_ServerId_bound: value_bound a object.(S2S_Gossip_Sending_ServerId))
-      (S2S_Gossip_Receiving_ServerId_bound: value_bound a object.(S2S_Gossip_Receiving_ServerId))
-      (S2S_Gossip_Operations_bound: value_bound a object.(S2S_Gossip_Operations))
-      (S2S_Gossip_Index_bound: value_bound a object.(S2S_Gossip_Index))
-      (S2S_Acknowledge_Gossip_Sending_ServerId_bound: value_bound a object.(S2S_Acknowledge_Gossip_Sending_ServerId))
-      (S2S_Acknowledge_Gossip_Receiving_ServerId_bound: value_bound a object.(S2S_Acknowledge_Gossip_Receiving_ServerId))
-      (S2S_Acknowledge_Gossip_Index_bound: value_bound a object.(S2S_Acknowledge_Gossip_Index))
-      (S2C_Client_OperationType_bound: value_bound 1 object.(S2C_Client_OperationType))
-      (S2C_Client_VersionVector_bound: value_bound a object.(S2C_Client_VersionVector))
-      (S2C_Server_Id_bound: value_bound a object.(S2C_Server_Id))
-      (S2C_Client_Number: value_bound a object.(S2C_Client_Number))
-      : _value_bound object.
-
-  #[global]
-  Instance has_value_boundary : has_value_boundary (t u64) :=
-    @_value_bound.
+  Definition value_bound (msg: Message.t) : Prop :=
+    u64_le_CONSTANT msg.(Message.MessageType) /\ u64_le_CONSTANT msg.(Message.C2S_Client_Id) /\ u64_le_CONSTANT msg.(Message.C2S_Server_Id) /\ u64_le_CONSTANT msg.(Message.C2S_Client_OperationType) /\ Forall u64_le_CONSTANT msg.(Message.C2S_Client_VersionVector) /\ u64_le_CONSTANT msg.(Message.S2S_Gossip_Sending_ServerId) /\ u64_le_CONSTANT msg.(Message.S2S_Gossip_Index) /\ u64_le_CONSTANT msg.(Message.S2S_Acknowledge_Gossip_Sending_ServerId) /\ u64_le_CONSTANT msg.(Message.S2S_Acknowledge_Gossip_Receiving_ServerId) /\ u64_le_CONSTANT msg.(Message.S2S_Acknowledge_Gossip_Index) /\ u64_le_CONSTANT msg.(Message.S2C_Client_OperationType) /\ Forall u64_le_CONSTANT msg.(Message.S2C_Client_VersionVector) /\ u64_le_CONSTANT msg.(Message.S2C_Server_Id) /\ u64_le_CONSTANT msg.(Message.S2C_Server_Id).
 
   End ADD_ON.
 
 End Message.
+
+#[global] Hint Unfold Message.size_of : session_hints.
+#[global] Hint Unfold Message.value_bound : session_hints.
 
 Module Server.
 
@@ -289,36 +263,18 @@ Module Server.
     end.
 
   Definition val (v: tuple_of tv) : val :=
-    SessionPrelude.value_of v.
+    tuple_of_has_value_of tv v.
 
-  #[projections(primitive), universes(template)]
-  Record t {u64: Type} : Type := mk
+  Record t : Type := mk
     { Id:                     u64
     ; NumberOfServers:        u64
-    ; UnsatisfiedRequests:    list (Message.t u64)
+    ; UnsatisfiedRequests:    list (Message.t)
     ; VectorClock:            list u64
-    ; OperationsPerformed:    list (Operation.t u64)
-    ; MyOperations:           list (Operation.t u64)
-    ; PendingOperations:      list (Operation.t u64)
+    ; OperationsPerformed:    list (Operation.t)
+    ; MyOperations:           list (Operation.t)
+    ; PendingOperations:      list (Operation.t)
     ; GossipAcknowledgements: list u64
     }.
-
-  #[global] Arguments t : clear implicits.
-
-  #[global]
-  Instance FMap
-    : FMap Server.t.
-  Proof.
-    intros A B A_to_B F_A. econstructor.
-    - refine (A_to_B _). refine (Id _). exact F_A.
-    - refine (A_to_B _). refine (NumberOfServers _). exact F_A.
-    - refine (fmap (Message.FMap A B A_to_B) _). refine (UnsatisfiedRequests _). exact F_A.
-    - refine (fmap A_to_B _). refine (VectorClock _). exact F_A.
-    - refine (fmap (Operation.FMap A B A_to_B) _). refine (OperationsPerformed _). exact F_A.
-    - refine (fmap (Operation.FMap A B A_to_B) _). refine (MyOperations _). exact F_A.
-    - refine (fmap (Operation.FMap A B A_to_B) _). refine (PendingOperations _). exact F_A.
-    - refine (fmap A_to_B _). refine (GossipAcknowledgements _). exact F_A.
-  Qed.
 
   #[global, program]
   Instance IntoVal : IntoVal (tuple_of tv) :=
@@ -330,34 +286,34 @@ Module Server.
     tac_IntoVal 7.
   Defined.
 
+  Theorem val_t v
+    : val_ty (Server.val v) (struct.t SessionServer.Server).
+  Proof.
+    tac_val_t.
+  Qed.
+
+  #[global] Hint Resolve val_t : core.
+
+  #[global] Instance Session_IntoValForType
+    : IntoValForType (tuple_of tv) (struct.t SessionServer.Server).
+  Proof.
+    tac_IntoValForType.
+  Qed.
+
   Section ADD_ON.
 
-  Context {u64: Type}.
+  Definition size_of (server: Server.t) : nat * nat * nat * nat * nat :=
+    (length server.(VectorClock), length server.(OperationsPerformed), length server.(MyOperations), length server.(PendingOperations), length server.(GossipAcknowledgements)).
 
-  Definition size_of (object: t u64) : nat * nat * nat * nat * nat :=
-    (length object.(VectorClock), length object.(OperationsPerformed), length object.(MyOperations), length object.(PendingOperations), length object.(GossipAcknowledgements)).
-
-  Context `(has_value_boundary u64).
-
-  Variant _value_bound {a: Z} (object: t u64) : Prop :=
-    | _value_bound_intro
-      (Id_bound: value_bound a object.(Id))
-      (NumberOfServers_bound: value_bound a object.(NumberOfServers))
-      (UnsatisfiedRequests_bound: value_bound a object.(UnsatisfiedRequests))
-      (VectorClock_bound: value_bound a object.(VectorClock))
-      (OperationsPerformed_bound: value_bound a object.(OperationsPerformed))
-      (MyOperations_bound: value_bound a object.(MyOperations))
-      (PendingOperations_bound: value_bound a object.(PendingOperations))
-      (GossipAcknowledgements_bound: value_bound a object.(GossipAcknowledgements))
-      : _value_bound object.
-
-  #[global]
-  Instance has_value_boundary : has_value_boundary (t u64) :=
-    @_value_bound.
+  Definition value_bound (server: Server.t) : Prop :=
+    u64_le_CONSTANT server.(Server.Id) /\ u64_le_CONSTANT server.(Server.NumberOfServers) /\ Forall u64_le_CONSTANT server.(Server.VectorClock).
 
   End ADD_ON.
 
 End Server.
+
+#[global] Hint Unfold Server.size_of : session_hints.
+#[global] Hint Unfold Server.value_bound : session_hints.
 
 Module Client.
 
@@ -375,30 +331,16 @@ Module Client.
     end.
 
   Definition val (v: tuple_of tv) : val :=
-    SessionPrelude.value_of v.
+    tuple_of_has_value_of tv v.
 
-  #[projections(primitive), universes(template)]
-  Record t {u64: Type} : Type := mk
+  #[projections(primitive)]
+  Record t : Type := mk
     { Id:                 u64
     ; NumberOfServers:    u64
     ; WriteVersionVector: list u64
     ; ReadVersionVector:  list u64
     ; SessionSemantic:    u64
     }.
-
-  #[global] Arguments t : clear implicits.
-
-  #[global]
-  Instance FMap
-    : FMap Client.t.
-  Proof.
-    intros A B A_to_B F_A. econstructor.
-    - refine (A_to_B _). refine (Id _). exact F_A.
-    - refine (A_to_B _). refine (NumberOfServers _). exact F_A.
-    - refine (fmap A_to_B _). refine (WriteVersionVector _). exact F_A.
-    - refine (fmap A_to_B _). refine (ReadVersionVector _). exact F_A.
-    - refine (A_to_B _). refine (SessionSemantic _). exact F_A.
-  Defined.
 
   #[global, program]
   Instance IntoVal : IntoVal (tuple_of tv) :=
@@ -410,89 +352,61 @@ Module Client.
     tac_IntoVal 4.
   Defined.
 
+  Theorem val_t v
+    : val_ty (Client.val v) (struct.t SessionClient.Client).
+  Proof.
+    tac_val_t.
+  Qed.
+
+  #[global] Hint Resolve val_t : core.
+
+  #[global] Instance Client_IntoValForType
+    : IntoValForType (tuple_of tv) (struct.t SessionClient.Client).
+  Proof.
+    tac_IntoValForType.
+  Qed.
+
   Section ADD_ON.
 
-  Context {u64: Type}.
+  Definition size_of (client: Client.t) : nat * nat :=
+    (length client.(WriteVersionVector), length client.(ReadVersionVector)).
 
-  Definition size_of (object: t u64) : nat * nat :=
-    (length object.(WriteVersionVector), length object.(ReadVersionVector)).
-
-  Context `(has_value_boundary u64).
-
-  Variant _value_bound {a: Z} (object: t nat) : Prop :=
-    | _value_bound_intro
-      (Id_bound: value_bound a object.(Id))
-      (NumberOfServers_bound: value_bound a object.(NumberOfServers))
-      (WriteVersionVector_bound: value_bound a object.(WriteVersionVector))
-      (ReadVersionVector_bound: value_bound a object.(ReadVersionVector))
-      (SessionSemantic_bound: value_bound 1 object.(SessionSemantic))
-      : _value_bound object.
-
-  #[global]
-  Instance has_value_boundary : has_value_boundary (t nat) :=
-    @_value_bound.
+  Definition value_bound (client: Client.t) : Prop :=
+    u64_le_CONSTANT client.(Client.Id) /\ u64_le_CONSTANT client.(Client.NumberOfServers) /\ Forall u64_le_CONSTANT client.(Client.WriteVersionVector) /\ Forall u64_le_CONSTANT client.(Client.ReadVersionVector).
 
   End ADD_ON.
 
 End Client.
 
+#[global] Hint Unfold Client.size_of : session_hints.
+#[global] Hint Unfold Client.value_bound : session_hints.
+
 Module ServerSide.
 
   Include SessionServer.
-
-  Theorem Operation_val_t v
-    : val_ty (Operation.val v) (struct.t SessionServer.Operation).
-  Proof.
-    tac_val_t.
-  Qed.
-
-  #[global] Hint Resolve Operation_val_t : typeclasses_hints.
-
-  Theorem Message_val_t v
-    : val_ty (Message.val v) (struct.t SessionServer.Message).
-  Proof.
-    tac_val_t.
-  Qed.
-
-  #[global] Hint Resolve Message_val_t : typeclasses_hints.
-
-  Theorem Server_val_t v
-    : val_ty (Server.val v) (struct.t SessionServer.Server).
-  Proof.
-    tac_val_t.
-  Qed.
-
-  #[global] Hint Resolve Server_val_t : typeclasses_hints.
 
   Section heap.
 
   Context `{hG: !heapGS Σ}.
 
-  #[local] Notation operation := (Operation.t u64).
-  #[local] Notation operationList := (list operation).
-  #[local] Notation message := (Message.t u64).
-  #[local] Notation messageList := (list message).
-  #[local] Notation server := (Server.t u64).
-
-  Definition isOperation (v: tuple_of Operation.tv) (op: operation) (n: nat) : iProp Σ :=
+  Definition is_operation (v: tuple_of Operation.tv) (op: Operation.t) (n: nat) : iProp Σ :=
     own_slice_small v!(0) uint64T DfracDiscarded op.(Operation.VersionVector) ∗
     ⌜v!(1) = op.(Operation.Data)⌝ ∗
-    ⌜Operation.size_of op = n⌝.
+    ⌜Operation.size_of op = n /\ Operation.value_bound op⌝.
 
-  Definition isOperationSlice (s: Slice.t) (ops: operationList) (n: nat) : iProp Σ :=
-    ∃ vs, own_slice s (struct.t Operation) (DfracOwn 1) vs ∗ [∗ list] v;op ∈ vs;ops, isOperation v op n.
+  Definition operation_slice (s: Slice.t) (ops: list Operation.t) (n: nat) : iProp Σ :=
+    ∃ vs, own_slice s (struct.t Operation) (DfracOwn 1) vs ∗ [∗ list] v;op ∈ vs;ops, is_operation v op n.
 
-  Definition isMessage (v: tuple_of Message.tv) (msg: message) (n: nat) (len_c2s: nat) (len_s2c: nat) : iProp Σ :=
+  Definition is_message (v: tuple_of Message.tv) (msg: Message.t) (n: nat) (len_c2s: nat) (len_s2c: nat) : iProp Σ :=
     ⌜v!(0) = msg.(Message.MessageType)⌝ ∗
     ⌜v!(1) = msg.(Message.C2S_Client_Id)⌝ ∗
     ⌜v!(2) = msg.(Message.C2S_Server_Id)⌝ ∗
     ⌜v!(3) = msg.(Message.C2S_Client_OperationType)⌝ ∗
     ⌜v!(4) = msg.(Message.C2S_Client_Data)⌝ ∗
     own_slice_small v!(5) uint64T (DfracOwn 1) msg.(Message.C2S_Client_VersionVector) ∗
-    ⌜len_c2s = length msg.(Message.C2S_Client_VersionVector)⌝ ∗
     ⌜v!(6) = msg.(Message.S2S_Gossip_Sending_ServerId)⌝ ∗
     ⌜v!(7) = msg.(Message.S2S_Gossip_Receiving_ServerId)⌝ ∗
-    isOperationSlice v!(8) msg.(Message.S2S_Gossip_Operations) n ∗
+    operation_slice v!(8) msg.(Message.S2S_Gossip_Operations) n ∗
     ⌜v!(9) = msg.(Message.S2S_Gossip_Index)⌝ ∗
     ⌜v!(10) = msg.(Message.S2S_Acknowledge_Gossip_Sending_ServerId)⌝ ∗
     ⌜v!(11) = msg.(Message.S2S_Acknowledge_Gossip_Receiving_ServerId)⌝ ∗
@@ -502,31 +416,28 @@ Module ServerSide.
     own_slice_small v!(15) uint64T (DfracOwn 1) msg.(Message.S2C_Client_VersionVector) ∗
     ⌜v!(16) = msg.(Message.S2C_Server_Id)⌝ ∗
     ⌜v!(17) = msg.(Message.S2C_Client_Number)⌝ ∗
-    ⌜Message.size_of msg = (len_c2s, len_s2c)⌝.
+    ⌜Message.size_of msg = (len_c2s, len_s2c) /\ Message.value_bound msg⌝.
 
-  Definition isMessageSlice (s: Slice.t) (msgs: messageList) (n: nat) (len_c2s: nat) : iProp Σ :=
-    ∃ vs, own_slice s (struct.t Message) (DfracOwn 1) vs ∗ [∗ list] v;msg ∈ vs;msgs, ∃ len_s2c : nat, isMessage v msg n len_c2s len_s2c.
+  Definition message_slice (s: Slice.t) (msgs: list Message.t) (n: nat) (len_c2s: nat) : iProp Σ :=
+    ∃ vs, own_slice s (struct.t server.Message) (DfracOwn 1) vs ∗ [∗ list] v;msg ∈ vs;msgs, ∃ len_s2c : nat, is_message v msg n len_c2s len_s2c.
 
-  Definition isServer' {OWN_UnsatisfiedRequests: bool} (v: tuple_of Server.tv) (server: server) (n: nat) (len_vc: nat) (len_op: nat) (len_mo: nat) (len_po: nat) (len_ga: nat) : iProp Σ :=
+  Definition is_server' (v: tuple_of Server.tv) (server: Server.t) (n: nat) (len_vc: nat) (len_op: nat) (len_mo: nat) (len_po: nat) (len_ga: nat) (OWN_UnsatisfiedRequests: bool) : iProp Σ :=
     ⌜v!(0) = server.(Server.Id)⌝ ∗
     ⌜v!(1) = server.(Server.NumberOfServers)⌝ ∗
-    (if OWN_UnsatisfiedRequests then isMessageSlice v!(2) server.(Server.UnsatisfiedRequests) n len_vc else emp)%I ∗
+    (if OWN_UnsatisfiedRequests then message_slice v!(2) server.(Server.UnsatisfiedRequests) n len_vc else emp)%I ∗
     own_slice_small v!(3) uint64T (DfracOwn 1) server.(Server.VectorClock) ∗
-    isOperationSlice v!(4) server.(Server.OperationsPerformed) len_op ∗
-    isOperationSlice v!(5) server.(Server.MyOperations) len_mo ∗
-    isOperationSlice v!(6) server.(Server.PendingOperations) len_po ∗
+    operation_slice v!(4) server.(Server.OperationsPerformed) len_op ∗
+    operation_slice v!(5) server.(Server.MyOperations) len_mo ∗
+    operation_slice v!(6) server.(Server.PendingOperations) len_po ∗
     own_slice_small v!(7) uint64T (DfracOwn 1) server.(Server.GossipAcknowledgements) ∗
-    ⌜Server.size_of server = (len_vc, len_op, len_mo, len_po, len_ga)⌝.
+    ⌜Server.size_of server = (len_vc, len_op, len_mo, len_po, len_ga) /\ Server.value_bound server⌝.
+
+  Definition is_server sv s n len_vc len_op len_mo len_po len_ga : iProp Σ :=
+    is_server' sv s n len_vc len_op len_mo len_po len_ga true.
 
   End heap.
 
-  Notation isServer := (isServer' (OWN_UnsatisfiedRequests := true)).
-
-  Section Coq_nat.
-
-  #[local] Notation Operation := (Operation.t u64).
-  #[local] Notation Message := (Message.t u64).
-  #[local] Notation Server := (Server.t u64).
+  Section Coq_u64.
 
   Fixpoint coq_compareVersionVector (v1: list u64) (v2: list u64) : bool :=
     match v1 with
@@ -585,15 +496,18 @@ Module ServerSide.
       end
     end.
 
-  Variant binarySearch_spec (needle: Operation) (l: list Operation) (n: nat) (RESULT: nat) : Prop :=
-    | binarySearch_spec_intro (prefix: list (list u64)) (suffix: list (list u64))
+  Definition coq_equalOperations (o1: Operation.t) (o2: Operation.t) : bool :=
+    coq_equalSlices o1.(Operation.VersionVector) o2.(Operation.VersionVector) && (uint.Z o1.(Operation.Data) =? uint.Z (o2.(Operation.Data))).
+
+  Variant binarySearch_spec (needle: Operation.t) (l: list Operation.t) (n: nat) (RESULT: nat) : Prop :=
+    | binarySearch_spec_intro prefix suffix
       (LENGTH: RESULT = length prefix)
       (VECTOR: map Operation.getVersionVector l = if forallb (fun x => negb (coq_equalSlices x.(Operation.VersionVector) needle.(Operation.VersionVector))) l then prefix ++ suffix else prefix ++ [Operation.getVersionVector needle] ++ suffix)
       (PREFIX: ∀ op, In op prefix -> coq_lexicographicCompare needle.(Operation.VersionVector) op = true)
       (SUFFIX: ∀ op, In op suffix -> coq_lexicographicCompare op needle.(Operation.VersionVector) = true)
       : binarySearch_spec needle l n RESULT.
 
-  Fixpoint coq_sortedInsert (l: list Operation) (i: Operation) : list Operation :=
+  Fixpoint coq_sortedInsert (l: list Operation.t) (i: Operation.t) : list Operation.t :=
     match l with
     | [] => [i]
     | h :: t =>
@@ -605,19 +519,25 @@ Module ServerSide.
         h :: coq_sortedInsert t i
     end.
 
-  Definition coq_getDataFromOperationLog (l: list Operation) : u64 :=
+  Definition coq_deleteAtIndexOperation (o: list Operation.t) (index: nat) : list Operation.t :=
+    take index o ++ drop (index + 1)%nat o.
+
+  Definition coq_deleteAtIndexMessage (m: list Message.t) (index: nat) : list Message.t :=
+    take index m ++ drop (index + 1)%nat m.
+
+  Definition coq_getDataFromOperationLog (l: list Operation.t) : u64 :=
     match last l with
     | Some v => v.(Operation.Data)
     | None => W64 0
     end.
 
-  Definition coq_receiveGossip (server: Server) (request: Message) : Server :=
+  Definition coq_receiveGossip (server: Server.t) (request: Message.t) : Server.t :=
     if (length request.(Message.S2S_Gossip_Operations) =? 0)%nat then
       server
     else
-      let first_loop_output : Server :=
+      let first_loop_output : Server.t :=
         let focus := request.(Message.S2S_Gossip_Operations) in
-        let loop_step (acc: Server) (elem: Operation) : Server :=
+        let loop_step (acc: Server.t) (elem: Operation.t) : Server.t :=
           let server := acc in
           if coq_oneOffVersionVector server.(Server.VectorClock) elem.(Operation.VersionVector) then
             {|
@@ -647,21 +567,21 @@ Module ServerSide.
         fold_left loop_step focus server
       in
       let server := first_loop_output in
-      let second_loop_output : Server * u64 * list u64 :=
+      let second_loop_output : Server.t * u64 * list u64 :=
         let focus := server.(Server.PendingOperations) in
-        let loop_step (acc: Server * u64 * list u64) (elem: Operation) : Server * u64 * list u64 :=
+        let loop_step (acc: Server.t * u64 * list u64) (elem: Operation.t) : Server.t * u64 * list u64 :=
           let '(server, i, seen) := acc in
             if coq_oneOffVersionVector server.(Server.VectorClock) elem.(Operation.VersionVector) then
-              (Server.mk u64 server.(Server.Id) server.(Server.NumberOfServers) server.(Server.UnsatisfiedRequests) (coq_maxTS server.(Server.VectorClock) elem.(Operation.VersionVector)) (coq_sortedInsert server.(Server.OperationsPerformed) elem) server.(Server.MyOperations) server.(Server.PendingOperations) server.(Server.GossipAcknowledgements), W64 (uint.Z i + 1), seen ++ [i])
+              (Server.mk server.(Server.Id) server.(Server.NumberOfServers) server.(Server.UnsatisfiedRequests) (coq_maxTS server.(Server.VectorClock) elem.(Operation.VersionVector)) (coq_sortedInsert server.(Server.OperationsPerformed) elem) server.(Server.MyOperations) server.(Server.PendingOperations) server.(Server.GossipAcknowledgements), W64 (uint.Z i + 1), seen ++ [i])
             else
               (server, W64 (uint.Z i + 1), seen)
         in
         fold_left loop_step focus (server, W64 0, [])
       in
       let '(server, _, seen) := second_loop_output in
-      let third_loop_output : nat * nat * list Operation :=
+      let third_loop_output : nat * nat * list Operation.t :=
         let focus := server.(Server.PendingOperations) in
-        let loop_step (acc: nat * nat * list Operation) (elem: Operation) : nat * nat * list Operation :=
+        let loop_step (acc: nat * nat * list Operation.t) (elem: Operation.t) : nat * nat * list Operation.t :=
           let '(i, j, output) := acc in
           match seen !! j with
           | Some i' => if (i =? uint.nat i')%nat then ((i + 1)%nat, (j + 1)%nat, output) else ((i + 1)%nat, j, output ++ [elem])
@@ -682,7 +602,7 @@ Module ServerSide.
         Server.GossipAcknowledgements := server.(Server.GossipAcknowledgements);
       |}.
 
-  Definition coq_acknowledgeGossip (s: Server) (r: Message) : Server :=
+  Definition coq_acknowledgeGossip (s: Server.t) (r: Message.t) : Server.t :=
     let i := uint.nat (r.(Message.S2S_Acknowledge_Gossip_Sending_ServerId)) in
     let l := s.(Server.GossipAcknowledgements) in
     if (i >=? length l)%nat then
@@ -696,37 +616,40 @@ Module ServerSide.
       in
       let newGossipAcknowledgements := coq_maxTwoInts prevGossipAcknowledgementsValue r.(Message.S2S_Acknowledge_Gossip_Index) in
       let gossipAcknowledgements := <[i := newGossipAcknowledgements]> l in
-      Server.mk u64 s.(Server.Id) s.(Server.NumberOfServers) s.(Server.UnsatisfiedRequests) s.(Server.VectorClock) s.(Server.OperationsPerformed) s.(Server.MyOperations) s.(Server.PendingOperations) gossipAcknowledgements.
+      Server.mk s.(Server.Id) s.(Server.NumberOfServers) s.(Server.UnsatisfiedRequests) s.(Server.VectorClock) s.(Server.OperationsPerformed) s.(Server.MyOperations) s.(Server.PendingOperations) gossipAcknowledgements.
 
-  Definition coq_getGossipOperations (s: Server) (serverId: u64) : list Operation :=
+  Definition coq_getGossipOperations (s: Server.t) (serverId: u64) : list Operation.t :=
     match s.(Server.GossipAcknowledgements) !! uint.nat serverId with
     | Some v => drop (uint.nat v) s.(Server.MyOperations)
     | None => []
     end.
 
-  Definition coq_processClientRequest (s: Server) (r: Message) : bool * Server * Message :=
+  Definition coq_processClientRequest (s: Server.t) (r: Message.t) : bool * Server.t * Message.t :=
     if negb (coq_compareVersionVector s.(Server.VectorClock) r.(Message.C2S_Client_VersionVector)) then
-      (false, s, Message.mk u64 0 0 0 0 (IntoVal_def _Data.t) [] 0 0 [] 0 0 0 0 0 (IntoVal_def _Data.t) [] 0 0)
+      (false, s, Message.mk 0 0 0 0 (IntoVal_def _Data.t) [] 0 0 [] 0 0 0 0 0 (IntoVal_def _Data.t) [] 0 0)
     else
       if uint.Z r.(Message.C2S_Client_OperationType) =? 0 then
         let S2C_Client_Data := coq_getDataFromOperationLog s.(Server.OperationsPerformed) in
         let S2C_Client_VersionVector := s.(Server.VectorClock) in
         let S2C_Client_Number := r.(Message.C2S_Client_Id) in
         let S2C_Server_Id := s.(Server.Id) in
-        (true, s, Message.mk u64 4 0 0 0 (IntoVal_def _Data.t) [] 0 0 [] 0 0 0 0 0 S2C_Client_Data S2C_Client_VersionVector S2C_Server_Id S2C_Client_Number)
+        (true, s, Message.mk 4 0 0 0 (IntoVal_def _Data.t) [] 0 0 [] 0 0 0 0 0 S2C_Client_Data S2C_Client_VersionVector S2C_Server_Id S2C_Client_Number)
       else
         let v := match s.(Server.VectorClock) !! uint.nat s.(Server.Id) with Some v => uint.Z v | None => 0 end in
-        let VectorClock := <[uint.nat s.(Server.Id) := W64 (v + 1)]> s.(Server.VectorClock) in
-        let OperationsPerformed := coq_sortedInsert s.(Server.OperationsPerformed) (Operation.mk u64 VectorClock r.(Message.C2S_Client_Data)) in
-        let MyOperations := coq_sortedInsert s.(Server.MyOperations) (Operation.mk u64 VectorClock r.(Message.C2S_Client_Data)) in
-        let S2C_Client_OperationType := 1 in
-        let S2C_Client_Data := (IntoVal_def _Data.t) in
-        let S2C_Client_VersionVector := VectorClock in
-        let S2C_Client_Number := r.(Message.C2S_Client_Id) in
-        let S2C_Server_Id := s.(Server.Id) in
-        (true, Server.mk u64 s.(Server.Id) s.(Server.NumberOfServers) s.(Server.UnsatisfiedRequests) VectorClock OperationsPerformed MyOperations s.(Server.PendingOperations) s.(Server.GossipAcknowledgements), Message.mk u64 4 0 0 0 (IntoVal_def _Data.t) [] 0 0 [] 0 0 0 0 1 S2C_Client_Data S2C_Client_VersionVector S2C_Server_Id S2C_Client_Number).
+        if (v <=? CONSTANT - 1)%Z && (length s.(Server.MyOperations) <=? CONSTANT - 1)%Z then
+          let VectorClock := <[uint.nat s.(Server.Id) := W64 (v + 1)]> s.(Server.VectorClock) in
+          let OperationsPerformed := coq_sortedInsert s.(Server.OperationsPerformed) (Operation.mk VectorClock r.(Message.C2S_Client_Data)) in
+          let MyOperations := coq_sortedInsert s.(Server.MyOperations) (Operation.mk VectorClock r.(Message.C2S_Client_Data)) in
+          let S2C_Client_OperationType := 1 in
+          let S2C_Client_Data := (IntoVal_def _Data.t) in
+          let S2C_Client_VersionVector := VectorClock in
+          let S2C_Client_Number := r.(Message.C2S_Client_Id) in
+          let S2C_Server_Id := s.(Server.Id) in
+          (true, Server.mk s.(Server.Id) s.(Server.NumberOfServers) s.(Server.UnsatisfiedRequests) VectorClock OperationsPerformed MyOperations s.(Server.PendingOperations) s.(Server.GossipAcknowledgements), Message.mk 4 0 0 0 (IntoVal_def _Data.t) [] 0 0 [] 0 0 0 0 1 S2C_Client_Data S2C_Client_VersionVector S2C_Server_Id S2C_Client_Number)
+        else
+          (false, s, Message.mk 0 0 0 0 (IntoVal_def _Data.t) [] 0 0 [] 0 0 0 0 0 (IntoVal_def _Data.t) [] 0 0).
 
-  Definition coq_processRequest (server: Server) (request: Message) : Server * list Message :=
+  Definition coq_processRequest (server: Server.t) (request: Message.t) : Server.t * list Message.t :=
     match uint.nat request.(Message.MessageType) with
     | 0%nat =>
       let '(succeeded, server, reply) := coq_processClientRequest server request in
@@ -734,20 +657,20 @@ Module ServerSide.
         (server, [reply])
       else
         let UnsatisfiedRequests := server.(Server.UnsatisfiedRequests) ++ [request] in 
-        let server := Server.mk u64 server.(Server.Id) server.(Server.NumberOfServers) UnsatisfiedRequests server.(Server.VectorClock) server.(Server.OperationsPerformed) server.(Server.MyOperations) server.(Server.PendingOperations) server.(Server.GossipAcknowledgements) in
+        let server := Server.mk server.(Server.Id) server.(Server.NumberOfServers) UnsatisfiedRequests server.(Server.VectorClock) server.(Server.OperationsPerformed) server.(Server.MyOperations) server.(Server.PendingOperations) server.(Server.GossipAcknowledgements) in
         (server, [])
     | 1%nat =>
       let server := coq_receiveGossip server request in
       let focus := server.(Server.UnsatisfiedRequests) in
-      let loop_init : nat * Server * list Message :=
+      let loop_init : nat * Server.t * list Message.t :=
         (0%nat, server, [])
       in
-      let loop_step (acc: nat * Server * list Message) (element: Message) : nat * Server * list Message :=
+      let loop_step (acc: nat * Server.t * list Message.t) (element: Message.t) : nat * Server.t * list Message.t :=
         let '(i, s, outGoingRequests) := acc in
         let '(succeeded, s, reply) := coq_processClientRequest s element in
         if succeeded then
-          let UnsatisfiedRequests := SessionPrelude.deleteAt s.(Server.UnsatisfiedRequests) i in
-          (i, Server.mk u64 s.(Server.Id) s.(Server.NumberOfServers) UnsatisfiedRequests s.(Server.VectorClock) s.(Server.OperationsPerformed) s.(Server.MyOperations) s.(Server.PendingOperations) s.(Server.GossipAcknowledgements), outGoingRequests ++ [reply])
+          let UnsatisfiedRequests := coq_deleteAtIndexMessage s.(Server.UnsatisfiedRequests) i in
+          (i, Server.mk s.(Server.Id) s.(Server.NumberOfServers) UnsatisfiedRequests s.(Server.VectorClock) s.(Server.OperationsPerformed) s.(Server.MyOperations) s.(Server.PendingOperations) s.(Server.GossipAcknowledgements), outGoingRequests ++ [reply])
         else
           ((i + 1)%nat, s, outGoingRequests)
       in
@@ -755,7 +678,7 @@ Module ServerSide.
       (server, outGoingRequests)
     | 2%nat => (coq_acknowledgeGossip server request, [])
     | 3%nat =>
-      let loop_step (acc: Server * list Message) (index: u64) : Server * list Message :=
+      let loop_step (acc: Server.t * list Message.t) (index: u64) : Server.t * list Message.t :=
         let '(server, outGoingRequests) := acc in
         let operations := coq_getGossipOperations server index in
         if negb (uint.nat index =? uint.nat server.(Server.Id))%nat && negb (length operations =? 0)%nat then
@@ -764,8 +687,8 @@ Module ServerSide.
           let S2S_Gossip_Receiving_ServerId := index in
           let S2S_Gossip_Operations := operations in
           let S2S_Gossip_Index := length (server.(Server.MyOperations)) in
-          let message := Message.mk u64 1 0 0 0 (IntoVal_def _Data.t) [] S2S_Gossip_Sending_ServerId S2S_Gossip_Receiving_ServerId S2S_Gossip_Operations S2S_Gossip_Index 0 0 0 0 (IntoVal_def _Data.t) [] 0 0 in
-          (Server.mk u64 server.(Server.Id) server.(Server.NumberOfServers) server.(Server.UnsatisfiedRequests) server.(Server.VectorClock) server.(Server.OperationsPerformed) server.(Server.MyOperations) server.(Server.PendingOperations) GossipAcknowledgements, outGoingRequests ++ [message])
+          let message := Message.mk 1 0 0 0 (IntoVal_def _Data.t) [] S2S_Gossip_Sending_ServerId S2S_Gossip_Receiving_ServerId S2S_Gossip_Operations S2S_Gossip_Index 0 0 0 0 (IntoVal_def _Data.t) [] 0 0 in
+          (Server.mk server.(Server.Id) server.(Server.NumberOfServers) server.(Server.UnsatisfiedRequests) server.(Server.VectorClock) server.(Server.OperationsPerformed) server.(Server.MyOperations) server.(Server.PendingOperations) GossipAcknowledgements, outGoingRequests ++ [message])
         else
           (server, outGoingRequests)
       in
@@ -777,7 +700,7 @@ Module ServerSide.
     | _ => (server, [])
     end.
 
-  End Coq_nat.
+  End Coq_u64.
 
 End ServerSide.
 
@@ -785,55 +708,17 @@ Module ClientSide.
 
   Include SessionClient.
 
-  Theorem Operation_val_t v
-    : val_ty (Operation.val v) (struct.t SessionClient.Operation).
-  Proof.
-    exact (ServerSide.Operation_val_t v).
-  Defined.
-
-  #[global] Hint Resolve Operation_val_t : typeclasses_hints.
-
-  Theorem Message_val_t v
-    : val_ty (Message.val v) (struct.t SessionClient.Message).
-  Proof.
-    exact (ServerSide.Message_val_t v).
-  Defined.
-
-  #[global] Hint Resolve Message_val_t : typeclasses_hints.
-
-  Theorem Client_val_t v
-    : val_ty (Client.val v) (struct.t SessionClient.Client).
-  Proof.
-    tac_val_t.
-  Defined.
-
-  #[global] Hint Resolve Client_val_t : typeclasses_hints.
-
-  Notation isOperation := ServerSide.isOperation.
-
-  Notation isOperationSlice := ServerSide.isOperationSlice.
-
-  Notation isMessage := ServerSide.isMessage.
-
-  Notation isMessageSlice := ServerSide.isMessageSlice.
-
   Section heap.
 
   Context `{hG: !heapGS Σ}.
 
-  #[local] Notation operation := (Operation.t u64).
-  #[local] Notation operationList := (list operation).
-  #[local] Notation message := (Message.t u64).
-  #[local] Notation messageList := (list message).
-  #[local] Notation client := (Client.t u64).
-
-  Definition Client_u64 (v: tuple_of Client.tv) (client: client) (n: nat) : iProp Σ :=
+  Definition is_client (v: tuple_of Client.tv) (client: Client.t) (n: nat) : iProp Σ :=
     ⌜v!(0) = client.(Client.Id)⌝ ∗
     ⌜v!(1) = client.(Client.NumberOfServers)⌝ ∗
     own_slice_small v!(2) uint64T (DfracOwn 1) client.(Client.WriteVersionVector) ∗
     own_slice_small v!(3) uint64T (DfracOwn 1) client.(Client.ReadVersionVector) ∗
     ⌜v!(4) = client.(Client.SessionSemantic)⌝ ∗
-    ⌜(Client.size_of client, uint.nat client.(Client.NumberOfServers)) = (n, n, n)⌝.
+    ⌜(Client.size_of client, uint.nat client.(Client.NumberOfServers)) = (n, n, n) /\ Client.value_bound client⌝.
 
   End heap.
 
@@ -841,43 +726,39 @@ Module ClientSide.
 
   Import ServerSide.
 
-  #[local] Notation Operation := (Operation.t u64).
-  #[local] Notation Message := (Message.t u64).
-  #[local] Notation Client := (Client.t u64).
-
-  Definition coq_read (c: Client) (serverId: u64) : Message :=
+  Definition coq_read (c: Client.t) (serverId: u64) : Message.t :=
     match uint.nat c.(Client.SessionSemantic) with
-    | 0%nat => Message.mk u64 0 c.(Client.Id) serverId 0 (IntoVal_def _Data.t) (replicate (uint.nat c.(Client.NumberOfServers)) (W64 0)) 0 0 [] 0 0 0 0 0 (IntoVal_def _Data.t) [] 0 0
-    | 1%nat => Message.mk u64 0 c.(Client.Id) serverId 0 (IntoVal_def _Data.t) (replicate (uint.nat c.(Client.NumberOfServers)) (W64 0)) 0 0 [] 0 0 0 0 0 (IntoVal_def _Data.t) [] 0 0
-    | 2%nat => Message.mk u64 0 c.(Client.Id) serverId 0 (IntoVal_def _Data.t) (replicate (uint.nat c.(Client.NumberOfServers)) (W64 0)) 0 0 [] 0 0 0 0 0 (IntoVal_def _Data.t) [] 0 0
-    | 3%nat => Message.mk u64 0 c.(Client.Id) serverId 0 (IntoVal_def _Data.t) c.(Client.ReadVersionVector) 0 0 [] 0 0 0 0 0 (IntoVal_def _Data.t) [] 0 0
-    | 4%nat => Message.mk u64 0 c.(Client.Id) serverId 0 (IntoVal_def _Data.t) c.(Client.WriteVersionVector) 0 0 [] 0 0 0 0 0 (IntoVal_def _Data.t) [] 0 0
-    | 5%nat => Message.mk u64 0 c.(Client.Id) serverId 0 (IntoVal_def _Data.t) (coq_maxTS c.(Client.WriteVersionVector) c.(Client.ReadVersionVector)) 0 0 [] 0 0 0 0 0 (IntoVal_def _Data.t) [] 0 0
-    | _ => Message.mk u64 0 0 0 0 (IntoVal_def _Data.t) [] 0 0 [] 0 0 0 0 0 (IntoVal_def _Data.t) [] 0 0
+    | 0%nat => Message.mk 0 c.(Client.Id) serverId 0 (IntoVal_def _Data.t) (replicate (uint.nat c.(Client.NumberOfServers)) (W64 0)) 0 0 [] 0 0 0 0 0 (IntoVal_def _Data.t) [] 0 0
+    | 1%nat => Message.mk 0 c.(Client.Id) serverId 0 (IntoVal_def _Data.t) (replicate (uint.nat c.(Client.NumberOfServers)) (W64 0)) 0 0 [] 0 0 0 0 0 (IntoVal_def _Data.t) [] 0 0
+    | 2%nat => Message.mk 0 c.(Client.Id) serverId 0 (IntoVal_def _Data.t) (replicate (uint.nat c.(Client.NumberOfServers)) (W64 0)) 0 0 [] 0 0 0 0 0 (IntoVal_def _Data.t) [] 0 0
+    | 3%nat => Message.mk 0 c.(Client.Id) serverId 0 (IntoVal_def _Data.t) c.(Client.ReadVersionVector) 0 0 [] 0 0 0 0 0 (IntoVal_def _Data.t) [] 0 0
+    | 4%nat => Message.mk 0 c.(Client.Id) serverId 0 (IntoVal_def _Data.t) c.(Client.WriteVersionVector) 0 0 [] 0 0 0 0 0 (IntoVal_def _Data.t) [] 0 0
+    | 5%nat => Message.mk 0 c.(Client.Id) serverId 0 (IntoVal_def _Data.t) (coq_maxTS c.(Client.WriteVersionVector) c.(Client.ReadVersionVector)) 0 0 [] 0 0 0 0 0 (IntoVal_def _Data.t) [] 0 0
+    | _ => Message.mk 0 0 0 0 (IntoVal_def _Data.t) [] 0 0 [] 0 0 0 0 0 (IntoVal_def _Data.t) [] 0 0
     end.
 
-  Definition coq_write (c: Client) (serverId: u64) (value: u64) : Message :=
+  Definition coq_write (c: Client.t) (serverId: u64) (value: _Data.t) : Message.t :=
     match uint.nat c.(Client.SessionSemantic) with
-    | 0%nat => Message.mk u64 0 c.(Client.Id) serverId 1 value (replicate (uint.nat c.(Client.NumberOfServers)) (W64 0)) 0 0 [] 0 0 0 0 0 (IntoVal_def _Data.t) [] 0 0
-    | 1%nat => Message.mk u64 0 c.(Client.Id) serverId 1 value c.(Client.ReadVersionVector) 0 0 [] 0 0 0 0 0 (IntoVal_def _Data.t) [] 0 0
-    | 2%nat => Message.mk u64 0 c.(Client.Id) serverId 1 value c.(Client.WriteVersionVector) 0 0 [] 0 0 0 0 0 (IntoVal_def _Data.t) [] 0 0
-    | 3%nat => Message.mk u64 0 c.(Client.Id) serverId 1 value (replicate (uint.nat c.(Client.NumberOfServers)) (W64 0)) 0 0 [] 0 0 0 0 0 (IntoVal_def _Data.t) [] 0 0
-    | 4%nat => Message.mk u64 0 c.(Client.Id) serverId 1 value (replicate (uint.nat c.(Client.NumberOfServers)) (W64 0)) 0 0 [] 0 0 0 0 0 (IntoVal_def _Data.t) [] 0 0
-    | 5%nat => Message.mk u64 0 c.(Client.Id) serverId 1 value (coq_maxTS c.(Client.WriteVersionVector) c.(Client.ReadVersionVector)) 0 0 [] 0 0 0 0 0 (IntoVal_def _Data.t) [] 0 0
-    | _ => Message.mk u64 0 0 0 0 (IntoVal_def _Data.t) [] 0 0 [] 0 0 0 0 0 (IntoVal_def _Data.t) [] 0 0
+    | 0%nat => Message.mk 0 c.(Client.Id) serverId 1 value (replicate (uint.nat c.(Client.NumberOfServers)) (W64 0)) 0 0 [] 0 0 0 0 0 (IntoVal_def _Data.t) [] 0 0
+    | 1%nat => Message.mk 0 c.(Client.Id) serverId 1 value c.(Client.ReadVersionVector) 0 0 [] 0 0 0 0 0 (IntoVal_def _Data.t) [] 0 0
+    | 2%nat => Message.mk 0 c.(Client.Id) serverId 1 value c.(Client.WriteVersionVector) 0 0 [] 0 0 0 0 0 (IntoVal_def _Data.t) [] 0 0
+    | 3%nat => Message.mk 0 c.(Client.Id) serverId 1 value (replicate (uint.nat c.(Client.NumberOfServers)) (W64 0)) 0 0 [] 0 0 0 0 0 (IntoVal_def _Data.t) [] 0 0
+    | 4%nat => Message.mk 0 c.(Client.Id) serverId 1 value (replicate (uint.nat c.(Client.NumberOfServers)) (W64 0)) 0 0 [] 0 0 0 0 0 (IntoVal_def _Data.t) [] 0 0
+    | 5%nat => Message.mk 0 c.(Client.Id) serverId 1 value (coq_maxTS c.(Client.WriteVersionVector) c.(Client.ReadVersionVector)) 0 0 [] 0 0 0 0 0 (IntoVal_def _Data.t) [] 0 0
+    | _ => Message.mk 0 0 0 0 (IntoVal_def _Data.t) [] 0 0 [] 0 0 0 0 0 (IntoVal_def _Data.t) [] 0 0
     end.
 
-  Definition coq_processRequest (c: Client) (requestType: u64) (serverId: u64) (value: u64) (ackMessage: Message) : Client * Message :=
+  Definition coq_processRequest (c: Client.t) (requestType: u64) (serverId: u64) (value: _Data.t) (ackMessage: Message.t) : Client.t * Message.t :=
     match uint.nat requestType with
     | 0%nat => (c, coq_read c serverId)
     | 1%nat => (c, coq_write c serverId value)
     | 2%nat =>
       match uint.nat ackMessage.(Message.S2C_Client_OperationType) with
-      | 0%nat => (Client.mk u64 c.(Client.Id) c.(Client.NumberOfServers) c.(Client.WriteVersionVector) ackMessage.(Message.S2C_Client_VersionVector) c.(Client.SessionSemantic), Message.mk u64 0 0 0 0 (IntoVal_def _Data.t) [] 0 0 [] 0 0 0 0 0 (IntoVal_def _Data.t) [] 0 0)
-      | 1%nat => (Client.mk u64 c.(Client.Id) c.(Client.NumberOfServers) ackMessage.(Message.S2C_Client_VersionVector) c.(Client.ReadVersionVector) c.(Client.SessionSemantic), Message.mk u64 0 0 0 0 (IntoVal_def _Data.t) [] 0 0 [] 0 0 0 0 0 (IntoVal_def _Data.t) [] 0 0)
-      | _ => (c, Message.mk u64 0 0 0 0 (IntoVal_def _Data.t) [] 0 0 [] 0 0 0 0 0 (IntoVal_def _Data.t) [] 0 0)
+      | 0%nat => (Client.mk c.(Client.Id) c.(Client.NumberOfServers) c.(Client.WriteVersionVector) ackMessage.(Message.S2C_Client_VersionVector) c.(Client.SessionSemantic), Message.mk 0 0 0 0 (IntoVal_def _Data.t) [] 0 0 [] 0 0 0 0 0 (IntoVal_def _Data.t) [] 0 0)
+      | 1%nat => (Client.mk c.(Client.Id) c.(Client.NumberOfServers) ackMessage.(Message.S2C_Client_VersionVector) c.(Client.ReadVersionVector) c.(Client.SessionSemantic), Message.mk 0 0 0 0 (IntoVal_def _Data.t) [] 0 0 [] 0 0 0 0 0 (IntoVal_def _Data.t) [] 0 0)
+      | _ => (c, Message.mk 0 0 0 0 (IntoVal_def _Data.t) [] 0 0 [] 0 0 0 0 0 (IntoVal_def _Data.t) [] 0 0)
       end
-    | _ => (c, Message.mk u64 0 0 0 0 (IntoVal_def _Data.t) [] 0 0 [] 0 0 0 0 0 (IntoVal_def _Data.t) [] 0 0)
+    | _ => (c, Message.mk 0 0 0 0 (IntoVal_def _Data.t) [] 0 0 [] 0 0 0 0 0 (IntoVal_def _Data.t) [] 0 0)
     end.
 
   End Coq_nat.
@@ -888,20 +769,35 @@ Section properties.
 
 Import ServerSide SessionPrelude.
 
-Lemma redefine_coq_lexicographicCompare
-  : coq_lexicographicCompare = vectorGt.
+Lemma Forall_CONSTANT_replicate n
+  : Forall u64_le_CONSTANT (replicate n (W64 0)).
+Proof.
+  induction n as [ | n IH]; simpl; econstructor; eauto. eapply CONSTANT_ge_0.
+Qed.
+
+Lemma CONSTANT_coq_maxTs xs ys
+  (H_xs : Forall u64_le_CONSTANT xs)
+  (H_ys : Forall u64_le_CONSTANT ys)
+  : Forall u64_le_CONSTANT (coq_maxTS xs ys).
+Proof.
+  revert ys H_ys; induction H_xs as [ | x xs H_x H_xs IH]; intros ys H_ys; destruct H_ys as [ | y ys H_y H_ys]; simpl in *; try congruence; econstructor; simpl; eauto.
+  unfold coq_maxTwoInts. red in H_x, H_y |- *. rewrite -> CONSTANT_unfold in *. rewrite Z.gtb_ltb. destruct (_ <? _) as [ | ] eqn: H_OBS; [rewrite Z.ltb_lt in H_OBS | rewrite Z.ltb_nlt in H_OBS]; word.
+Qed.
+
+Lemma redefine_coq_lexicographicCompare :
+  coq_lexicographicCompare = vectorGt.
 Proof.
   reflexivity.
 Defined.
 
-Lemma redefine_coq_equalSlices
-  : coq_equalSlices = vectorEq.
+Lemma redefine_coq_equalSlices :
+  coq_equalSlices = vectorEq.
 Proof.
   reflexivity.
 Defined.
 
-Lemma redefine_coq_sortedInsert (n: nat)
-  : coq_sortedInsert = sortedInsert (hsOrd := Operation.hsOrd n).
+Lemma redefine_coq_sortedInsert (n : nat) :
+  coq_sortedInsert = sortedInsert (hsOrd := Operation.hsOrd n).
 Proof.
   reflexivity.
 Defined.
@@ -1015,17 +911,17 @@ Proof.
   - rewrite <- ltb_lt in H_gt; eauto 2. simpl in *. congruence.
 Qed.
 
-Definition is_sorted (l: list (Operation.t u64)) : Prop :=
+Definition is_sorted (l: list Operation.t) : Prop :=
   ∀ i, ∀ j, (i < j)%nat -> ∀ o1, ∀ o2, l !! i = Some o1 -> l !! j = Some o2 ->
   coq_lexicographicCompare o2.(Operation.VersionVector) o1.(Operation.VersionVector) = true.
 
-Lemma redefine_is_sorted n l
-  : is_sorted l = isSorted (hsOrd := Operation.hsOrd n) l.
+Lemma redefine_is_sorted (n: nat) (l: list Operation.t)
+  : is_sorted l = SessionPrelude.isSorted (hsOrd := Operation.hsOrd n) l.
 Proof.
   reflexivity.
 Defined.
 
-Lemma length_coq_maxTS n xs ys
+Lemma coq_maxTS_length n xs ys
   (LEN1: length xs = n)
   (LEN2: length ys = n)
   : length (coq_maxTS xs ys) = n.
@@ -1041,54 +937,31 @@ Proof.
   destruct (coq_equalSlices _ _) as [ | ]; simpl; try word.
 Qed.
 
-Lemma BOUND_replicate a x n
-  (BOUND_x : u64_has_value_boundary a x)
-  : Forall (u64_has_value_boundary a) (replicate n x).
-Proof.
-  induction n as [ | n IH]; simpl in *; eauto.
-Qed.
-
-Lemma BOUND_coq_maxTwoInts a x y
-  (BOUND_x : u64_has_value_boundary a x)
-  (BOUND_y : u64_has_value_boundary a y)
-  : u64_has_value_boundary a (coq_maxTwoInts x y).
-Proof.
-  unfold coq_maxTwoInts. red in BOUND_x, BOUND_y |- *. destruct (_ >? _)%Z as [ | ]; word.
-Qed.
-
-Lemma BOUND_coq_maxTS a xs ys
-  (BOUND_xs : Forall (u64_has_value_boundary a) xs)
-  (BOUND_ys : Forall (u64_has_value_boundary a) ys)
-  : Forall (u64_has_value_boundary a) (coq_maxTS xs ys).
-Proof.
-  revert ys BOUND_ys. induction BOUND_xs as [ | x x_wf xs xs_wf IH]; intros; destruct BOUND_ys as [ | y y_wf ys ys_wf]; simpl; eauto.
-  econstructor; eauto. eapply BOUND_coq_maxTwoInts; eauto.
-Qed.
-
 End properties.
 
 Module INVARIANT.
 
-  Variant WEAK_SERVER_INVARIANT (EXTRA: Server.t u64 -> Prop) (server: Server.t u64) : Prop :=
+  Variant WEAK_SERVER_INVARIANT (EXTRA: Server.t -> Prop) (s: Server.t) : Prop :=
     | WEAK_SERVER_INVARIANT_INTRO
-      (PendingOperations_is_sorted: is_sorted server.(Server.PendingOperations))
-      (OperationsPerformed_is_sorted: is_sorted server.(Server.OperationsPerformed))
-      (EXTRA_SERVER_INVARIANT: EXTRA server)
-      : WEAK_SERVER_INVARIANT EXTRA server.
+      (PendingOperations_is_sorted: is_sorted s.(Server.PendingOperations))
+      (OperationsPerformed_is_sorted: is_sorted s.(Server.OperationsPerformed))
+      (EXTRA_SERVER_INVARIANT: EXTRA s)
+      : WEAK_SERVER_INVARIANT EXTRA s.
 
-  Record SERVER_INVARIANT (EXTRA: Server.t u64 -> Prop) (server: Server.t u64) : Prop :=
+  Record SERVER_INVARIANT (EXTRA: Server.t -> Prop) (s: Server.t) : Prop :=
     SERVER_INVARIANT_INTRO
-    { PendingOperations_is_sorted: is_sorted server.(Server.PendingOperations)
-    ; OperationsPerformed_is_sorted: is_sorted server.(Server.OperationsPerformed)
-    ; MyOperations_is_sorted: is_sorted server.(Server.MyOperations)
-    ; Id_in_range: (uint.Z server.(Server.Id) >= 0)%Z /\ (uint.nat server.(Server.Id) < length server.(Server.VectorClock))%nat
-    ; EXTRA_SERVER_INVARIANT: EXTRA server
+    { PendingOperations_is_sorted: is_sorted s.(Server.PendingOperations)
+    ; OperationsPerformed_is_sorted: is_sorted s.(Server.OperationsPerformed)
+    ; MyOperations_is_sorted: is_sorted s.(Server.MyOperations)
+    ; Id_in_range: (uint.Z s.(Server.Id) >= 0)%Z /\ (uint.nat s.(Server.Id) < length s.(Server.VectorClock))%nat
+    ; EXTRA_SERVER_INVARIANT: EXTRA s
     }.
 
-  Record CLIENT_INVARIANT (EXTRA: Client.t u64 -> Prop) (client: Client.t u64) : Prop :=
+  Record CLIENT_INVARIANT (EXTRA: Client.t -> Prop) (c: Client.t) : Prop :=
     CLIENT_INVARIANT_INTRO
-    { SessionSemantic_le_5: (uint.nat client.(Client.SessionSemantic) <= 5)%nat
-    ; EXTRA_CLIENT_INVARIANT: EXTRA client
+    { SessionSemantic_ge_0: (uint.Z c.(Client.SessionSemantic) >= 0)%Z
+    ; SessionSemantic_le_5: (uint.Z c.(Client.SessionSemantic) <= 5)%Z
+    ; EXTRA_CLIENT_INVARIANT: EXTRA c
     }.
 
 End INVARIANT.
@@ -1097,21 +970,27 @@ Notation WEAK_SERVER_INVARIANT := INVARIANT.WEAK_SERVER_INVARIANT.
 Notation SERVER_INVARIANT := INVARIANT.SERVER_INVARIANT.
 Notation CLIENT_INVARIANT := INVARIANT.CLIENT_INVARIANT.
 
+Definition FINAL_SERVER_INVARIANT {n: nat} : Server.t -> Prop :=
+  let EXTRA_SERVER_INVARIANT (s: Server.t) : Prop :=
+    uint.nat s.(Server.NumberOfServers) = n /\ length s.(Server.GossipAcknowledgements) = n /\ (Z.of_nat (length s.(Server.MyOperations)) <= CONSTANT)%Z
+  in
+  SERVER_INVARIANT EXTRA_SERVER_INVARIANT.
+
 Section heap.
 
 Import ServerSide.
 
 Context `{hG: !heapGS Σ}.
 
-Lemma Operation_well_formed (n: nat) v op
-  : (isOperation v op n)%I ⊢@{iProp Σ} (⌜Operation.well_formed (u64_well_formed := fun _ => True) n op⌝)%I.
+Lemma Operation_well_formed op v (n : nat)
+  : (is_operation v op n)%I ⊢@{iProp Σ} (⌜Operation.well_formed n op⌝)%I.
 Proof.
-  iIntros "H_hd". iDestruct "H_hd" as "(H3 & %H2 & %H1)"; iClear "H3".
-  iPureIntro; split; [eapply SessionPrelude.Forall_True | done].
+  iIntros "H_hd". iDestruct "H_hd" as "(H3 & %H2 & %H1 & %H1')"; iClear "H3".
+  iPureIntro; split; [eapply SessionPrelude.Forall_True | eauto].
 Qed.
 
-Lemma Forall_Operation_well_formed (n: nat) vs ops
-  : ([∗ list] v;op ∈ vs;ops, isOperation v op n)%I ⊢@{iProp Σ} (⌜Forall (Operation.well_formed (u64_well_formed := fun _ => True) n) ops⌝)%I.
+Lemma Forall_Operation_wf ops vs (n: nat)
+  : ([∗ list] v;op ∈ vs;ops, is_operation v op n)%I ⊢@{iProp Σ} (⌜Forall (Operation.well_formed n) ops⌝)%I.
 Proof.
   revert vs; induction ops as [ | hd tl IH]; intros vs.
   - iIntros "H_big_sepL2"; iPureIntro; eauto.
@@ -1124,28 +1003,28 @@ Proof.
     iPureIntro; econstructor; trivial.
 Qed.
 
-Lemma VersionVector_length s ops n
-  : (isOperationSlice s ops n)%I ⊢@{iProp Σ} (⌜∀ i : nat, ∀ e, ops !! i = Some e -> length e.(Operation.VersionVector) = n⌝)%I.
+Lemma VersionVector_len (s: Slice.t) (ops: list Operation.t) (n: nat)
+  : (operation_slice s ops n)%I ⊢@{iProp Σ} (⌜∀ i : nat, ∀ e, ops !! i = Some e -> length e.(Operation.VersionVector) = n⌝)%I.
 Proof.
   iIntros "(%vs & H_vs & H)".
-  iPoseProof (Forall_Operation_well_formed with "H") as "%H_well_formed".
-  pose proof (List.Forall_forall (Operation.well_formed (u64_well_formed := fun _ => True) n) ops) as claim.
+  iPoseProof (Forall_Operation_wf with "H") as "%H_well_formed".
+  pose proof (List.Forall_forall (Operation.well_formed n) ops) as claim.
   rewrite claim in H_well_formed; iPureIntro; intros i x H_x.
-  enough (WTS: Operation.well_formed (u64_well_formed := fun _ => True) n x) by now red in WTS.
+  enough (WTS : Operation.well_formed n x) by now red in WTS.
   eapply H_well_formed; eapply SessionPrelude.lookup_In; eauto.
 Qed.
 
-Lemma pers_isOperation v op (n: nat)
-  : (isOperation v op n)%I ⊢@{iProp Σ} (<pers> (isOperation v op n))%I.
+Lemma pers_is_operation v op (n: nat)
+  : (is_operation v op n)%I ⊢@{iProp Σ} (<pers> (is_operation v op n))%I.
 Proof.
   iIntros "#H"; done.
 Qed.
 
-Lemma pers_big_sepL2_isOperation vs ops (n: nat)
-  : ([∗ list] v;op ∈ vs;ops, isOperation v op n)%I ⊢@{iProp Σ} (<pers> ([∗ list] v;op ∈ vs;ops, isOperation v op n))%I.
+Lemma pers_big_sepL2_is_operation ops vs (n: nat)
+  : ([∗ list] v;op ∈ vs;ops, is_operation v op n)%I ⊢@{iProp Σ} (<pers> ([∗ list] v;op ∈ vs;ops, is_operation v op n))%I.
 Proof.
   iIntros "H_big_sepL2"; iApply (big_sepL2_persistently).
-  iApply (big_sepL2_mono (λ k, λ y1, λ y2, isOperation y1 y2 n)%I with "[$H_big_sepL2]").
+  iApply (big_sepL2_mono (λ k, λ y1, λ y2, is_operation y1 y2 n)%I with "[$H_big_sepL2]").
   intros; iIntros "#H"; done.
 Qed.
 
@@ -1155,41 +1034,41 @@ Proof.
   iIntros "#H"; done.
 Qed.
 
-Lemma big_sepL2_isOperation_elim l ops (n: nat) (i: nat) l_i ops_i
-  (H_l_i: l !! i = Some l_i)
-  (H_ops_i: ops !! i = Some ops_i)
-  : ([∗ list] opv;o ∈ ops;l, isOperation opv o n)%I ⊢@{iProp Σ} (isOperation ops_i l_i n)%I.
+Lemma big_sepL2_is_operation_elim ops vs (n: nat) (i: nat) op v
+  (H_op: ops !! i = Some op)
+  (H_v: vs !! i = Some v)
+  : ([∗ list] v;op ∈ vs;ops, is_operation v op n)%I ⊢@{iProp Σ} (is_operation v op n)%I.
 Proof.
-  rewrite <- take_drop with (l := l) (i := i); rewrite <- take_drop with (l := ops) (i := i); iIntros "H". 
-  assert (i < length l)%nat as H1_i by now eapply lookup_lt_is_Some_1.
-  assert (i < length ops)%nat as H2_i by now eapply lookup_lt_is_Some_1.  
-  iAssert (([∗ list] opv;o ∈ take i ops;take i l, isOperation opv o n) ∗ ([∗ list] opv;o ∈ drop i ops;drop i l, isOperation opv o n))%I with "[H]" as "[H1 H2]".
+  rewrite <- take_drop with (l := ops) (i := i); rewrite <- take_drop with (l := vs) (i := i); iIntros "H". 
+  assert (i < length ops)%nat as H1_i by now eapply lookup_lt_is_Some_1.
+  assert (i < length vs)%nat as H2_i by now eapply lookup_lt_is_Some_1.  
+  iAssert (([∗ list] v;op ∈ take i vs;take i ops, is_operation v op n) ∗ ([∗ list] v;op ∈ drop i vs;drop i ops, is_operation v op n))%I with "[H]" as "[H1 H2]".
   { iApply (big_sepL2_app_equiv with "H"); do 2 rewrite length_take; word. }
-  destruct (drop i ops) as [ | ops_i' ops_suffix] eqn: H_ops_suffix.
-  { apply f_equal with (f := length) in H_ops_suffix; simpl in *; rewrite length_drop in H_ops_suffix. word. }
-  iPoseProof (big_sepL2_cons_inv_l with "[$H2]") as "(%l_i' & %l_suffix & %H_l_suffix & H3 & H4)".
-  rewrite <- take_drop with (l := l) (i := i) in H_l_i; rewrite <- take_drop with (l := ops) (i := i) in H_ops_i.
-  rewrite H_l_suffix in H_l_i; rewrite H_ops_suffix in H_ops_i.
-  assert (i = length (take i l)) as H3_i.
+  destruct (drop i vs) as [ | v' vs_suffix] eqn: H_vs_suffix.
+  { apply f_equal with (f := length) in H_vs_suffix; simpl in *; rewrite length_drop in H_vs_suffix. word. }
+  iPoseProof (big_sepL2_cons_inv_l with "[$H2]") as "(%op' & %ops_suffix & %H_ops_suffix & H3 & H4)".
+  rewrite <- take_drop with (l := ops) (i := i) in H_op; rewrite <- take_drop with (l := vs) (i := i) in H_v.
+  rewrite H_ops_suffix in H_op; rewrite H_vs_suffix in H_v.
+  assert (i = length (take i ops)) as H3_i.
   { rewrite length_take; word. }
-  assert (i = length (take i ops)) as H4_i.
+  assert (i = length (take i vs)) as H4_i.
   { rewrite length_take; word. }
-  pose proof (list_lookup_middle (take i l) l_suffix l_i' i H3_i) as EQ_l_i.
-  pose proof (list_lookup_middle (take i ops) ops_suffix ops_i' i H4_i) as EQ_ops_i.
-  assert (l_i = l_i' /\ ops_i = ops_i') as [<- <-] by now split; congruence.
+  pose proof (list_lookup_middle (take i ops) ops_suffix op' i H3_i) as EQ_l_i.
+  pose proof (list_lookup_middle (take i vs) vs_suffix v' i H4_i) as EQ_ops_i.
+  assert (op = op' /\ v = v') as [<- <-] by now split; congruence.
   iExact "H3".
 Qed.
 
-Lemma big_sepL2_isOperation_intro l ops n
-  (LENGTH: length l = length ops)
-  : (∀ i : nat, ∀ l_i, ∀ ops_i, ⌜(l !! i = Some l_i) /\ (ops !! i = Some ops_i)⌝ -∗ isOperation ops_i l_i n)%I ⊢@{iProp Σ} ([∗ list] opv;o ∈ ops;l, isOperation opv o n)%I.
+Lemma big_sepL2_is_operation_intro ops vs (n: nat)
+  (LENGTH: length ops = length vs)
+  : (∀ i : nat, ∀ op, ∀ v, ⌜(ops !! i = Some op) /\ (vs !! i = Some v)⌝ -∗ is_operation op v n)%I ⊢@{iProp Σ} ([∗ list] v;op ∈ vs;ops, is_operation op v n)%I.
 Proof.
-  revert ops n LENGTH; induction l as [ | l_hd l_tl IH], ops as [ | ops_hd ops_tl]; intros; simpl in *; try congruence.
+  revert vs n LENGTH; induction ops as [ | ops_hd ops_tl IH], vs as [ | v_hd v_tl]; intros; simpl in *; try congruence.
   - iIntros "#H"; iClear "H"; done.
   - iIntros "#H"; iSplit.
     + iApply "H"; instantiate (1 := 0%nat); done.
     + iApply IH. { word. }
-      iIntros "%i %l_i %ops_i [%H_l_i %H_ops_i]"; iApply "H"; instantiate (1 := S i); done.
+      iIntros "%i %op %v [%H_op %H_v]"; iApply "H"; instantiate (1 := S i); done.
 Qed.
 
 Lemma big_sepL2_middle_split {A: Type} {B: Type} {Φ: A -> B -> iProp Σ} {xs: list A} {i: nat} {x0: A} (ys: list B)
@@ -1217,11 +1096,8 @@ Proof.
   rewrite <- take_drop with (l := xs) (i := i) in claim1 at -1.
   apply SessionPrelude.app_cancel_l in claim1; rewrite take_drop in claim1.
   assert (x0' = x0) as -> by congruence.
-  iSplitL "H_middle".
-  { iExact "H_middle". }
-  rewrite take_drop; iSplitL "H_prefix".
-  { iExact "H_prefix". }
-  { rewrite <- drop_drop with (l := xs) (n1 := 1%nat) (n2 := i); rewrite -> EQ; iExact "H_suffix". }
+  iFrame; rewrite take_drop; iFrame.
+  rewrite <- drop_drop with (l := xs) (n1 := 1%nat) (n2 := i); rewrite -> EQ; iExact "H_suffix".
 Qed.
 
 Lemma big_sepL2_middle_merge {A: Type} {B: Type} {Φ: A -> B -> iProp Σ} {xs: list A} {i: nat} {x0: A} (y0: B) (ys1: list B) (ys2: list B)
